Generalize list_sort_elem to arbitrary types.

theories/examples/list_sort_elem.v
@@ -4,369 +4,269 @@ From iris.heap_lang Require Import proofmode notation.
 From iris.heap_lang Require Import assert.
 From osiris.utils Require Import list.
 
-Definition compareZ : val :=
-  λ: "x" "y", "x" ≤ "y".
-
 Definition cont := true.
 Definition stop := false.
 
 Definition list_sort_elem_service_split : val :=
   rec: "go" "c" "c1" "c2" :=
-    if: ~(recv "c")
-    then send "c1" #stop;; send "c2" #stop
-    else let: "x" := recv "c" in
-         send "c1" #cont;; send "c1" "x";; "go" "c" "c2" "c1".
+    if: ~(recv "c") then send "c1" #stop;; send "c2" #stop else
+    let: "x" := recv "c" in
+    send "c1" #cont;; send "c1" "x";;
+    "go" "c" "c2" "c1".
 
-Definition list_sort_elem_service_copy : val :=
+Definition list_sort_elem_service_move : val :=
   rec: "go" "c" "cin" :=
-    if: ~(recv "cin")
-    then send "c" #stop
-    else let: "x" := recv "cin" in send "c" #cont;; send "c" "x";; "go" "c" "cin".
+    if: ~(recv "cin") then send "c" #stop else
+    let: "x" := recv "cin" in
+    send "c" #cont;; send "c" "x";;
+    "go" "c" "cin".
 
 Definition list_sort_elem_service_merge : val :=
-  rec: "go" "c" "x1" "c1" "c2" :=
-    if: ~recv "c2"
-    then send "c" #cont;; send "c" "x1";; list_sort_elem_service_copy "c" "c1"
-    else let: "x2" := recv "c2" in
-         if: compareZ "x1" "x2"
-         then send "c" #cont;; send "c" "x1";; "go" "c" "x2" "c2" "c1"
-         else send "c" #cont;; send "c" "x2";; "go" "c" "x1" "c1" "c2".
+  rec: "go" "cmp" "c" "x1" "c1" "c2" :=
+    if: ~recv "c2" then
+      send "c" #cont;; send "c" "x1";;
+      list_sort_elem_service_move "c" "c1"
+    else
+      let: "x2" := recv "c2" in
+      if: "cmp" "x1" "x2" then
+        send "c" #cont;; send "c" "x1";; "go" "cmp" "c" "x2" "c2" "c1"
+      else
+        send "c" #cont;; send "c" "x2";; "go" "cmp" "c" "x1" "c1" "c2".
 
 Definition list_sort_elem_service : val :=
-  rec: "go" "c" :=
-    if: ~(recv "c")
-    then send "c" #stop
-    else let: "x" := recv "c" in
-         if: ~(recv "c")
-         then send "c" #cont;; send "c" "x";; send "c" #stop
-         else let: "y" := recv "c" in
-              let: "c1" := start_chan ("go") in
-              let: "c2" := start_chan ("go") in
-              send "c1" #cont;; send "c1" "x";;
-              send "c2" #cont;; send "c2" "y";;
-              list_sort_elem_service_split "c" "c1" "c2";;
-              let: "x" := (if: recv "c1" then recv "c1" else assert #false) in
-              list_sort_elem_service_merge "c" "x" "c1" "c2".
+  rec: "go" "cmp" "c" :=
+    if: ~(recv "c") then send "c" #stop else
+    let: "x" := recv "c" in
+    if: ~(recv "c") then send "c" #cont;; send "c" "x";; send "c" #stop else
+    let: "y" := recv "c" in
+    let: "c1" := start_chan (λ: "c", "go" "cmp" "c") in
+    let: "c2" := start_chan (λ: "c", "go" "cmp" "c") in
+    send "c1" #cont;; send "c1" "x";;
+    send "c2" #cont;; send "c2" "y";;
+    list_sort_elem_service_split "c" "c1" "c2";;
+    let: "x" := (if: recv "c1" then recv "c1" else assert #false) in
+    list_sort_elem_service_merge "cmp" "c" "x" "c1" "c2".
+
+(** This definition is also in list_sort, move elsewhere *)
+Definition cmp_spec `{!heapG Σ} {A} (I : A → val → iProp Σ)
+    (R : relation A) `{!RelDecision R} (cmp : val) : iProp Σ :=
+  (∀ x x' v v',
+    {{{ I x v ∗ I x' v' }}}
+      cmp v v'
+    {{{ RET #(bool_decide (R x x')); I x v ∗ I x' v' }}})%I.
 
 Section list_sort_elem.
   Context `{!heapG Σ, !proto_chanG Σ} (N : namespace).
+  Context {A} (I : A → val → iProp Σ) (R : relation A) `{!RelDecision R, !Total R}.
 
-  Definition tail_protocol_aux (rec : list Z -d> list Z -d> iProto Σ)
-    : (list Z -d> list Z -d> iProto Σ) :=
-    λ xs ys,
-    (<?> (b:bool), MSG #b
-        {{ if b then True else ⌜ ys ≡ₚ xs ⌝ }};
-      if b
-      then <?> (y:Z), MSG #y {{ ⌜ TlRel (≤) y ys ⌝ }}; (rec : _ -> _ -> iProto Σ) xs (ys++[y])
-      else END)%proto.
+  Definition tail_protocol_aux (xs : list (A * val))
+      (rec : list (A * val) -d> iProto Σ) : list (A * val) -d> iProto Σ := λ ys,
+    ((<?> y v, MSG v {{ ⌜ TlRel R y (fst <$> ys) ⌝ ∗ I y v }}; (rec : _ → iProto Σ) (ys ++ [(y,v)]))
+     <&{⌜ ys ≡ₚ xs ⌝}> END)%proto.
 
-  Instance tail_protocol_aux_contractive : Contractive (tail_protocol_aux).
+  Instance tail_protocol_aux_contractive xs : Contractive (tail_protocol_aux xs).
   Proof.
-    intros n p p' Hp. rewrite /tail_protocol_aux.
-    intros xs ys.
-    apply iProto_message_ne=> b //=.
-    destruct b.
-    - apply iProto_message_contractive=> //=.
-      intros x.
-      destruct n as [|n]; simpl in *; try done. apply Hp.
-    - done.
+    intros n p p' Hp ys. apply iProto_branch_ne=> //=.
+    apply iProto_message_contractive=> x //=. destruct n as [|n]=> //=.
   Qed.
-  
-  Definition tail_protocol : (list Z -d> list Z -d> iProto Σ) := fixpoint (tail_protocol_aux).
+  Definition tail_protocol (xs : list (A * val)) : list (A * val) → iProto Σ :=
+    fixpoint (tail_protocol_aux xs).
   Lemma tail_protocol_unfold xs ys:
-    tail_protocol xs ys≡ tail_protocol_aux tail_protocol xs ys.
-  Proof. apply (fixpoint_unfold tail_protocol_aux). Qed.
-  
-  Definition helper_protocol_aux (rec : list Z -d> iProto Σ)
-    : (list Z -d> iProto Σ) :=
-    λ xs,
-    (<!> (b:bool), MSG #b;
-       if b
-       then <!> (x:Z), MSG #x; (rec : _ → iProto Σ) (xs++[x])
-       else tail_protocol xs [])%proto.
-  
-  Instance helper_protocol_aux_contractive : Contractive (helper_protocol_aux).
+    tail_protocol xs ys ≡ tail_protocol_aux xs (tail_protocol xs) ys.
+  Proof. apply (fixpoint_unfold (tail_protocol_aux _)). Qed.
+
+  Definition head_protocol_aux
+      (rec : list (A * val) -d> iProto Σ) : list (A * val) -d> iProto Σ := λ xs,
+    ((<!> x v, MSG v {{ I x v }}; (rec : _ → iProto Σ) (xs ++ [(x,v)]))
+     <+> tail_protocol xs [])%proto.
+
+  Instance head_protocol_aux_contractive : Contractive head_protocol_aux.
   Proof.
-    intros n p p' Hp. rewrite /helper_protocol_aux.
-    intros xs.
-    apply iProto_message_ne=> b //=.
-    destruct b.
-    - apply iProto_message_contractive=> //=.
-      intros x.
-      destruct n as [|n]; simpl in *; done.
-    - done.
+    intros n p p' Hp xs. apply iProto_branch_ne=> //=.
+    apply iProto_message_contractive=> //= x. destruct n as [|n]=> //=.
   Qed.
 
-  Definition helper_protocol : (list Z -d> iProto Σ) := fixpoint (helper_protocol_aux).
-  Lemma helper_protocol_unfold xs :
-    helper_protocol xs ≡ helper_protocol_aux helper_protocol xs.
-  Proof. apply (fixpoint_unfold helper_protocol_aux). Qed.
+  Definition head_protocol : list (A * val) → iProto Σ := fixpoint head_protocol_aux.
+  Lemma head_protocol_unfold xs :
+    head_protocol xs ≡ head_protocol_aux head_protocol xs.
+  Proof. apply (fixpoint_unfold head_protocol_aux). Qed.
 
-  Definition list_sort_elem_protocol := helper_protocol [].
+  Definition list_sort_elem_protocol : iProto Σ := head_protocol [].
 
-  Lemma list_sort_elem_service_split_spec c c1 c2 (xs xs1 xs2 : list Z) :
+  Lemma list_sort_elem_service_split_spec c c1 c2 xs xs1 xs2 :
     {{{
-         c ↣ iProto_dual (helper_protocol xs) @ N ∗ 
-         c1 ↣ helper_protocol xs1 @ N ∗ 
-         c2 ↣ helper_protocol xs2 @ N
-     }}}
+      c ↣ iProto_dual (head_protocol xs) @ N ∗ 
+      c1 ↣ head_protocol xs1 @ N ∗ c2 ↣ head_protocol xs2 @ N
+    }}}
       list_sort_elem_service_split c c1 c2
     {{{ xs' xs1' xs2', RET #();
-        c ↣ iProto_dual (tail_protocol (xs++xs') []) @ N ∗
-        c1 ↣ tail_protocol (xs1++xs1') [] @ N ∗ 
-        c2 ↣ tail_protocol (xs2++xs2') [] @ N ∗
-        ⌜xs' ≡ₚ  xs1' ++ xs2'⌝
-      }}}.
+      ⌜xs' ≡ₚ xs1' ++ xs2'⌝ ∗
+      c ↣ iProto_dual (tail_protocol (xs ++ xs') []) @ N ∗
+     c1 ↣ tail_protocol (xs1 ++ xs1') [] @ N ∗ c2 ↣ tail_protocol (xs2 ++ xs2') [] @ N
+    }}}.
   Proof.
     iIntros (Ψ) "(Hc & Hc1 & Hc2) HΨ". iLöb as "IH" forall (c c1 c2 xs xs1 xs2 Ψ).
     wp_rec.
-    rewrite helper_protocol_unfold.
-    wp_apply (recv_proto_spec N with "Hc")=> //=.
-    iIntros (b) "Hc _".
-    destruct b.
-    - wp_apply (recv_proto_spec N with "Hc")=> //=.
-      iIntros (x) "Hc _".
-      wp_pures.
-      rewrite (helper_protocol_unfold xs1).
-      wp_apply (send_proto_spec N with "Hc1")=> //=.
-      iExists cont. iSplit; first done; iSplit; first done; iIntros "!> Hc1".
-      wp_apply (send_proto_spec N with "Hc1")=> //=.
-      iExists x. iSplit; first done; iSplit; first done; iIntros "!> Hc1".
-      wp_apply ("IH" with "[Hc] [Hc2] [Hc1]")=> //.
-      iIntros (xs' xs1' xs2') "(Hc & Hc2 & Hc1 & Hperm)".
-      iApply "HΨ".
-      iSplitL "Hc".
-      rewrite -app_assoc. rewrite -cons_middle. iApply "Hc".
-      iSplitL "Hc1".
-      rewrite -app_assoc. rewrite -cons_middle. iApply "Hc1".
-      iFrame.
-      iDestruct "Hperm" as %Hperm.
-      iPureIntro.
-      simpl. apply Permutation_cons.
-      rewrite Hperm.
-      apply Permutation_app_comm.
-    - rewrite (helper_protocol_unfold xs1).
-      wp_apply (send_proto_spec N with "Hc1")=> //=.
-      iExists stop. iSplit; first done; iSplit; first done; iIntros "!> Hc1".
-      rewrite (helper_protocol_unfold xs2).
-      wp_apply (send_proto_spec N with "Hc2")=> //=.
-      iExists stop. iSplit; first done; iSplit; first done; iIntros "!> Hc2".
-      iSpecialize ("HΨ" $![] [] []).
-      iApply "HΨ".
-      repeat rewrite app_nil_r.
-      iFrame.
-      done.
+    rewrite head_protocol_unfold.
+    wp_apply (branch_spec with "Hc"); iIntros ([]) "[Hc _]"; wp_pures.
+    - wp_apply (recv_proto_spec with "Hc"); iIntros (x v) "/= Hc HI".
+      rewrite (head_protocol_unfold xs1).
+      wp_apply (select_spec with "[$Hc1]")=> //=; iIntros "Hc1".
+      wp_apply (send_proto_spec with "Hc1"); simpl.
+      iExists x, v. iSplit; [done|]. iIntros "{$HI} !> Hc1".
+      wp_apply ("IH" with "Hc Hc2 Hc1").
+      iIntros (xs' xs1' xs2'); iDestruct 1 as (Hxs') "(Hc & Hc2 & Hc1)".
+      rewrite -!(assoc_L (++)).
+      iApply "HΨ". iFrame "Hc Hc1 Hc2". by rewrite Hxs' (comm (++) xs1') assoc_L.
+    - rewrite (head_protocol_unfold xs1) (head_protocol_unfold xs2).
+      wp_apply (select_spec with "[$Hc1]")=> //=; iIntros "Hc1".
+      wp_apply (select_spec with "[$Hc2]")=> //=; iIntros "Hc2".
+      iApply ("HΨ" $! [] [] []). rewrite !right_id_L. by iFrame.
   Qed.
 
-  Lemma cmp_spec :
-    (∀ x y,
-      {{{ True }}}
-        compareZ #x #y
-      {{{ RET #(bool_decide (x ≤ y)); True }}})%I.
-  Proof.
-    iIntros (x y Φ).
-    iModIntro. 
-    iIntros "_ HΦ".
-    wp_lam.
-    wp_pures.
-    by iApply "HΦ".
-  Qed.
-
-  Lemma list_sort_elem_service_copy_spec c cin xs ys zs xs' ys' :
-    xs ≡ₚ  xs' ++ zs →
-    ys ≡ₚ  ys' ++ zs →
-    Sorted (≤) ys →
-    (∀ x, TlRel Z.le x ys' → TlRel Z.le x ys) →
+  Lemma list_sort_elem_service_move_spec c cin xs ys zs xs' ys' :
+    xs ≡ₚ xs' ++ zs →
+    ys ≡ₚ ys' ++ zs →
+    Sorted R (fst <$> ys) →
+    (∀ x, TlRel R x (fst <$> ys') → TlRel R x (fst <$> ys)) →
     {{{
       c ↣ iProto_dual (tail_protocol xs ys) @ N ∗
       cin ↣ tail_protocol xs' ys' @ N
     }}}
-      list_sort_elem_service_copy c cin
+      list_sort_elem_service_move c cin
     {{{ RET #(); c ↣ END @ N ∗ cin ↣ END @ N }}}.
   Proof.
-    iIntros (H1 H2 Hsorted Hrel Ψ) "[Hc Hcin] HΨ".
-    iLöb as "IH" forall (c cin xs ys xs' ys' H1 H2 Hsorted Hrel).
+    iIntros (Hxs Hys Hsorted Hrel Ψ) "[Hc Hcin] HΨ".
+    iLöb as "IH" forall (c cin xs ys xs' ys' Hxs Hys Hsorted Hrel).
     wp_rec.
     rewrite (tail_protocol_unfold xs').
-    wp_apply (recv_proto_spec N with "Hcin")=> //=.
-    iIntros (b) "Hcin HP".
-    destruct b.
-    - iClear "HP".
-      wp_apply (recv_proto_spec N with "Hcin")=> //=.
-      iIntros (x) "Hcin".
-      iIntros (HP).
+    wp_apply (branch_spec with "Hcin"); iIntros ([]) "[Hcin Hys']".
+    - iClear "Hys'".
+      wp_apply (recv_proto_spec with "Hcin"); iIntros (x v) "/= Hcin".
+      iDestruct 1 as (Hx) "HI".
       rewrite (tail_protocol_unfold xs).
-      wp_apply (send_proto_spec N with "Hc")=> //=.
-      iExists cont. iSplit; first done; iSplit; first done; iIntros "!> Hc".
-      wp_apply (send_proto_spec N with "Hc")=> //=.
-      iExists x. iSplit; first done; iSplit; first by auto. iIntros "!> Hc".
-      wp_apply ("IH" with "[%] [%] [%] [%] Hc Hcin")=> //.
-      { by rewrite H2 -app_assoc -app_assoc (Permutation_app_comm zs). }
-      { apply Sorted_snoc; auto. }
-      { intros x'. inversion 1; discriminate_list || simplify_list_eq.
-          by constructor. }
-    - rewrite (tail_protocol_unfold xs).
-      wp_apply (send_proto_spec N with "Hc")=> //=.
-      iExists stop. iSplit; first done.
-      iDestruct "HP" as %HP.
-      simpl.
-      iSplit.
-      { by rewrite H1 -HP H2. }
-      iIntros "!> Hc".
-      iApply "HΨ".
-      iFrame.
-  Qed.
-    
-  Lemma list_sort_elem_service_merge_spec c c1 c2 xs ys xs1 xs2 y1 ys1 ys2 :
-    xs ≡ₚ xs1 ++ xs2 →
-    ys ≡ₚ ys1 ++ ys2 →
-    Sorted (≤) ys →
-    TlRel (≤) y1 ys →
-    (∀ x, TlRel Z.le x ys2 → x ≤ y1 → TlRel Z.le x ys) →
-    {{{
-      c ↣ iProto_dual (tail_protocol xs ys) @ N ∗ 
-      c1 ↣ tail_protocol xs1 (ys1 ++ [y1]) @ N ∗ 
-      c2 ↣ tail_protocol xs2 ys2 @ N
-    }}}
-      list_sort_elem_service_merge c #y1 c1 c2
-    {{{ RET #(); c ↣ END @ N ∗ c1 ↣ END @ N ∗ c2 ↣ END @ N}}}.
-  Proof.
-    iIntros (Hxs Hys Hsort Htl Htl_le Ψ) "(Hc & Hc1 & Hc2) HΨ".
-    iLöb as "IH" forall (c1 c2 xs1 xs2 ys y1 ys1 ys2 Hxs Hys Hsort Htl Htl_le).
-    wp_rec.
-    rewrite (tail_protocol_unfold xs).
-    rewrite (tail_protocol_unfold xs2).
-    wp_apply (recv_proto_spec N with "Hc2")=> //=.
-    iIntros (b) "Hc2 HP".
-    destruct b.
-    - iClear "HP".
-      wp_apply (recv_proto_spec N with "Hc2")=> //=.
-      iIntros (x) "Hc2"; iIntros (Htl2).
-      wp_pures.
-      wp_apply (cmp_spec)=> //. iIntros (_).
-      case_bool_decide.
-      + wp_apply (send_proto_spec N with "Hc")=> //=.
-        iExists cont. iSplit; first done; iSplit; first done; iIntros "!> Hc".
-        wp_apply (send_proto_spec N with "Hc")=> //=.
-        iExists y1. iSplit; first done. iSplit; first done.
-        iIntros "!> Hc".
-        wp_apply ("IH" with "[%] [%] [%] [%] [%] Hc Hc2 Hc1").
-        { by rewrite comm. }
-        { by rewrite assoc (comm _ ys2) Hys. }
-        { by apply Sorted_snoc. }
-        { by constructor. }
-        { intros x'. inversion 1; discriminate_list || simplify_list_eq.
-          constructor; lia. }
-        iIntros "(?&?&?)". iApply "HΨ"; iFrame.
-      + wp_apply (send_proto_spec N with "Hc")=> //=.
-        iExists cont. iSplit; first done; iSplit; first done; iIntros "!> Hc".
-        wp_apply (send_proto_spec N with "Hc")=> //=.
-        iExists x. iSplit; first done. iSplit.
-        { iPureIntro. auto with lia. }
-        iIntros "!> Hc".
-        wp_apply ("IH" with "[% //] [%] [%] [%] [%] Hc Hc1 Hc2 [$]").
-        { by rewrite Hys assoc. }
-        { apply Sorted_snoc; auto with lia. }
-        { constructor. lia. }
-        { intros x'. inversion 1; discriminate_list || simplify_list_eq.
-          constructor; lia. }
-    - wp_apply (send_proto_spec N with "Hc")=> //=.
-      iExists cont. iSplit; first done; iSplit; first done; iIntros "!> Hc".
-      wp_apply (send_proto_spec N with "Hc")=> //=.
-      iDestruct "HP" as %HP.
-      iExists y1. iSplit; first done; iSplit; first done; iIntros "!> Hc".
-      wp_apply (list_sort_elem_service_copy_spec with "[$Hc $Hc1]")=> //.
-      { by rewrite Hys -app_assoc -app_assoc (Permutation_app_comm [y1]) HP. }
-      { by apply Sorted_snoc. }
-      { intros x'. inversion 1; discriminate_list || simplify_list_eq.
-          constructor; lia. }
-      iIntros "[Hc Hc1]".
-      iApply "HΨ".
-      iFrame.
+      wp_apply (select_spec with "[$Hc]")=> //=; iIntros "Hc".
+      wp_apply (send_proto_spec with "Hc"); simpl.
+      iExists x, v. iFrame "HI". do 2 (iSplit; [by auto|]); iIntros "!> Hc".
+      wp_apply ("IH" with "[%] [%] [%] [%] Hc Hcin HΨ").
+      { done. }
+      { by rewrite Hys -!assoc_L (comm _ zs). }
+      { rewrite fmap_app /=. apply Sorted_snoc; auto. }
+      { intros x'. rewrite !fmap_app.
+        inversion 1; discriminate_list || simplify_list_eq. by constructor. }
+    - iDestruct "Hys'" as %Hys'. rewrite (tail_protocol_unfold xs).
+      wp_apply (select_spec with "[$Hc]")=> //=.
+      { by rewrite Hys Hxs Hys'. }
+      iIntros "Hc". iApply "HΨ". iFrame.
   Qed.
 
-  Lemma list_sort_elem_service_spec c :
+  Lemma list_sort_elem_service_merge_spec cmp c c1 c2 xs ys xs1 xs2 y1 w1 ys1 ys2 :
+    xs ≡ₚ xs1 ++ xs2 →
+    ys ≡ₚ ys1 ++ ys2 →
+    Sorted R (fst <$> ys) →
+    TlRel R y1 (fst <$> ys) →
+    (∀ x, TlRel R x (fst <$> ys2) → R x y1 → TlRel R x (fst <$> ys)) →
+    cmp_spec I R cmp -∗
+    {{{
+      c ↣ iProto_dual (tail_protocol xs ys) @ N ∗ 
+      c1 ↣ tail_protocol xs1 (ys1 ++ [(y1,w1)]) @ N ∗ c2 ↣ tail_protocol xs2 ys2 @ N ∗
+      I y1 w1
+    }}}
+      list_sort_elem_service_merge cmp c w1 c1 c2
+    {{{ RET #(); c ↣ END @ N ∗ c1 ↣ END @ N ∗ c2 ↣ END @ N }}}.
+  Proof.
+    iIntros (Hxs Hys Hsort Htl Htl_le) "#Hcmp !>".
+    iIntros (Ψ) "(Hc & Hc1 & Hc2 & HIy1) HΨ".
+    iLöb as "IH" forall (c1 c2 xs1 xs2 ys y1 w1 ys1 ys2 Hxs Hys Hsort Htl Htl_le).
+    wp_rec.
+    rewrite (tail_protocol_unfold xs) (tail_protocol_unfold xs2).
+    wp_apply (branch_spec with "[$Hc2]"); iIntros ([]) "[Hc2 Hys2]".
+    - iClear "Hys2".
+      wp_apply (recv_proto_spec with "Hc2"); iIntros (x v) "/= Hc2".
+      iDestruct 1 as (Htl2) "HIx".
+      wp_pures. wp_apply ("Hcmp" with "[$HIy1 $HIx]"); iIntros "[HIy1 HIx]".
+      case_bool_decide.
+      + wp_apply (select_spec with "[$Hc]")=> //=; iIntros "Hc".
+        wp_apply (send_proto_spec with "Hc"); simpl.
+        iExists y1, w1. iFrame "HIy1". do 2 (iSplit; [done|]); iIntros "!> Hc".
+        wp_apply ("IH" with "[%] [%] [%] [%] [%] Hc Hc2 Hc1 HIx").
+        { by rewrite comm. }
+        { by rewrite assoc (comm _ ys2) Hys. }
+        { rewrite fmap_app. by apply Sorted_snoc. }
+        { rewrite fmap_app. by constructor. }
+        { intros x'. rewrite !fmap_app.
+          inversion 1; discriminate_list || simplify_list_eq. by constructor. }
+        iIntros "(?&?&?)". iApply "HΨ"; iFrame.
+      + wp_apply (select_spec with "[$Hc]")=> //=; iIntros "Hc".
+        wp_apply (send_proto_spec with "Hc"); simpl.
+        iExists x, v. iFrame "HIx". iSplit; [done|]; iSplit.
+        { iPureIntro. by apply Htl_le, total_not. }
+        iIntros "!> Hc".
+        wp_apply ("IH" with "[% //] [%] [%] [%] [%] Hc Hc1 Hc2 HIy1 HΨ").
+        { by rewrite Hys assoc. }
+        { rewrite fmap_app. by apply Sorted_snoc, Htl_le, total_not. }
+        { rewrite fmap_app. constructor. by apply total_not. }
+        { intros x'. rewrite !fmap_app.
+          inversion 1; discriminate_list || simplify_list_eq. by constructor. }
+    - iDestruct "Hys2" as %Hys2.
+      wp_apply (select_spec with "[$Hc]")=> //=; iIntros "Hc".
+      wp_apply (send_proto_spec with "Hc"); simpl.
+      iExists y1, w1. iFrame "HIy1". do 2 (iSplit; [done|]); iIntros "!> Hc".
+      wp_apply (list_sort_elem_service_move_spec with "[$Hc $Hc1]").
+      { done. }
+      { by rewrite Hys Hys2 -!assoc_L (comm _ xs2). }
+      { rewrite fmap_app. by apply Sorted_snoc. }
+      { intros x'. rewrite !fmap_app.
+        inversion 1; discriminate_list || simplify_list_eq. by constructor. }
+      iIntros "[Hc Hc1]". iApply "HΨ". iFrame.
+  Qed.
+
+  Lemma list_sort_elem_service_spec cmp c :
+    cmp_spec I R cmp -∗
     {{{ c ↣ iProto_dual list_sort_elem_protocol @ N }}}
-      list_sort_elem_service c
+      list_sort_elem_service cmp c
     {{{ RET #(); c ↣ END @ N }}}.
   Proof.
-    iIntros (Ψ) "Hc HΨ". iLöb as "IH" forall (c Ψ).
-    wp_rec.
-    rewrite /list_sort_elem_protocol.
-    rewrite {2}helper_protocol_unfold.
-    wp_apply (recv_proto_spec N with "Hc")=> //=.
-    iIntros (b) "Hc _".
-    destruct b.
-    - wp_apply (recv_proto_spec N with "Hc")=> //=.
-      iIntros (x1) "Hc _".
-      rewrite (helper_protocol_unfold [x1]).
-      wp_apply (recv_proto_spec N with "Hc")=> //=.
-      iIntros (b) "Hc _".
-      destruct b.
-      + wp_apply (recv_proto_spec N with "[Hc]")=> //=.
-        iIntros (x2) "Hc _".
-        wp_apply (start_chan_proto_spec N (list_sort_elem_protocol)).
-        { iIntros (cy) "Hcy".
-          iApply ("IH" with "Hcy")=>//. iNext. iIntros "Hcy". done. }
+    iIntros "#Hcmp !>" (Ψ) "Hc HΨ". iLöb as "IH" forall (c Ψ).
+    wp_rec; wp_pures. rewrite /list_sort_elem_protocol {2}head_protocol_unfold.
+    wp_apply (branch_spec with "Hc"); iIntros ([]) "[Hc _]"; wp_pures.
+    - wp_apply (recv_proto_spec with "Hc"); iIntros (x1 v1) "/= Hc HIx1".
+      rewrite (head_protocol_unfold [_]).
+      wp_apply (branch_spec with "Hc"); iIntros ([]) "[Hc _]"; wp_pures.
+      + wp_apply (recv_proto_spec with "Hc"); iIntros (x2 v2) "/= Hc HIx2".
+        wp_apply (start_chan_proto_spec N list_sort_elem_protocol).
+        { iIntros (cy) "Hcy". wp_apply ("IH" with "Hcy"); auto. }
         iIntros (cy) "Hcy".
-        wp_apply (start_chan_proto_spec N (list_sort_elem_protocol)).
-        { iIntros (cz) "Hcz".
-          iApply ("IH" with "Hcz")=>//. iNext. iIntros "Hcz". done. }
+        wp_apply (start_chan_proto_spec N list_sort_elem_protocol).
+        { iIntros (cz) "Hcz". wp_apply ("IH" with "Hcz"); auto. }
         iIntros (cz) "Hcz".
-        rewrite /list_sort_elem_protocol.
-        rewrite {2}(helper_protocol_unfold []).
-        wp_apply (send_proto_spec N with "Hcy")=> //=.
-        iExists cont. iSplit; first done; iSplit; first done; iIntros "!> Hcy".
-        wp_apply (send_proto_spec N with "Hcy")=> //=.
-        iExists x1. iSplit; first done; iSplit; first done; iIntros "!> Hcy".
-        rewrite {2}(helper_protocol_unfold []).
-        wp_apply (send_proto_spec N with "Hcz")=> //=.
-        iExists cont. iSplit; first done; iSplit; first done; iIntros "!> Hcz".
-        wp_apply (send_proto_spec N with "Hcz")=> //=.
-        iExists x2. iSplit; first done; iSplit; first done; iIntros "!> Hcz".
-        wp_apply (list_sort_elem_service_split_spec with "[Hc Hcy Hcz]")=> //.
-        iFrame.
-        iIntros (xs' xs1' xs2') "(Hc & Hcy & Hcz & Hperm)".
-        iDestruct "Hperm" as %Hperm.
-        wp_pures.
-        rewrite (tail_protocol_unfold ([x1] ++ xs1')).
-        wp_apply (recv_proto_spec N with "[Hcy]")=> //=.
-        iIntros (b) "Hcy HP".
+        rewrite /list_sort_elem_protocol {2 3}(head_protocol_unfold []).
+        wp_apply (select_spec with "[$Hcy]")=> //; iIntros "Hcy".
+        wp_apply (send_proto_spec with "Hcy")=> //=.
+        iExists x1, v1. iFrame "HIx1". iSplit; [done|]; iIntros "!> Hcy".
+        wp_apply (select_spec with "[$Hcz]")=> //; iIntros "Hcz".
+        wp_apply (send_proto_spec with "Hcz")=> //=.
+        iExists x2, v2. iFrame "HIx2". iSplit; [done|]; iIntros "!> Hcz".
+        wp_apply (list_sort_elem_service_split_spec with "[$Hc $Hcy $Hcz]").
+        iIntros (xs' xs1' xs2'); iDestruct 1 as (Hxs') "(Hc & Hcy & Hcz) /=".
+        rewrite (tail_protocol_unfold (_ :: xs1')).
+        wp_apply (branch_spec with "Hcy"); iIntros (b) "[Hcy Hnil]".
         destruct b; last first.
-        { by iDestruct "HP" as %?%Permutation_nil_cons. }
-        iClear "HP".
-        wp_apply (recv_proto_spec N with "[Hcy]")=> //=.
-        iIntros (x) "Hcy _".
-        wp_apply (list_sort_elem_service_merge_spec _ _ _ _ [] _ _ _ [] []
-          with "[$Hc $Hcy $Hcz]"); auto using TlRel_nil.
-        { by rewrite /= Hperm Permutation_middle. }
-        iIntros "(Hc & Hcy & Hcz)".
-        by iApply "HΨ".
-      + rewrite (tail_protocol_unfold [x1] []).
-        wp_apply (send_proto_spec N with "[Hc]")=> //=.
-        iExists cont.
-        iSplitR=> //.
-        iSplitR=> //.
+        { by iDestruct "Hnil" as %?%Permutation_nil_cons. }
+        iClear "Hnil".
+        wp_apply (recv_proto_spec with "Hcy"); iIntros (x v) "/= Hcy [_ HIx]".
+        wp_apply (list_sort_elem_service_merge_spec _ _ _ _ _ [] _ _ _ _ [] []
+          with "Hcmp [$Hc $Hcy $Hcz $HIx]"); simpl; auto using TlRel_nil, Sorted_nil.
+        { by rewrite Hxs' Permutation_middle. }
+        iIntros "(Hc & Hcy & Hcz)". by iApply "HΨ".
+      + rewrite (tail_protocol_unfold [_]).
+        wp_apply (select_spec with "[$Hc]")=> //=; iIntros "Hc".
+        wp_apply (send_proto_spec with "Hc"); simpl.
+        iExists x1, v1. iFrame "HIx1". do 2 (iSplit; [by auto using TlRel_nil|]).
         iIntros "!> Hc".
-        wp_apply (send_proto_spec N with "[Hc]")=> //=.
-        iExists x1.
-        iSplitR=> //.
-        iSplitR; first by auto using TlRel_nil.
-        iIntros "!> Hc".
-        rewrite (tail_protocol_unfold [x1] [x1]).
-        wp_apply (send_proto_spec N with "[Hc]")=> //=.
-        iExists stop.
-        iSplitR=> //.
-        iSplitR=> //=.
-        iIntros "!> Hc". by iApply "HΨ".
-    - wp_pures.
-      rewrite (tail_protocol_unfold [] []).
-      wp_apply (send_proto_spec N with "[Hc]")=> //=.
-      iExists false.
-      iSplitR=>//.
-      iSplitR=>//.
-      iNext.
-      iIntros "Hc".
-      iApply "HΨ". iApply "Hc".
+        rewrite (tail_protocol_unfold [_]).
+        by wp_apply (select_spec with "[$Hc]").
+    - rewrite (tail_protocol_unfold []).
+      by wp_apply (select_spec with "[$Hc]").
   Qed.
 End list_sort_elem.
